Checkpoint definability proof.

Source/Definability.v
@@ -14,6 +14,10 @@ Import ListNotations.
 
 Import Source.
 
+Set Implicit Arguments.
+Unset Strict Implicit.
+Unset Printing Implicit Defensive.
+
 Section Definability.
   Variable p: program.
   Variable ictx: Program.interface.
@@ -80,22 +84,10 @@ Section Definability.
   Inductive state := State {
     (* Some P if the program is currently executing a context procedure P;
        otherwise None. *)
-    cur_proc : option Procedure.id;
+    cur_comp : option (Component.id * nat);
 
     (* Call stack with calling procedures. *)
-    callers  : list (option Procedure.id);
-
-    (* Function that maps component ids in the context to
-
-         (1) a counter indicating how many events that component has emitted
-             thus far, and;
-
-         (2) for each procedure in that component, the code it has executed thus
-             far.  This code is represented with a list of pairs (n, e) : Z *
-             expr.  The idea is that e is an expression that emits one of the
-             events encountered in the trace thus far, and n is how many events
-             were emitted earlier by that component. *)
-    procs    : PMap.t (Z * PMap.t (list (Z * expr)))
+    callers  : list (Component.id * nat)
 
   }.
 
@@ -104,91 +96,175 @@ Section Definability.
       procedure has no code.  Note that the actual current procedure takes into
       account whether mainC belongs to the context or not. *)
   Definition initial_state : state :=
-    let init_procs :=
-      PMap.map (fun procs =>
-                  (0%Z,
-                   fold_left (fun code_procs P => PMap.add P [] code_procs)
-                             (Component.export procs) (@PMap.empty _)))
-               ictx in
     match PMap.find mainC ictx with
-    | Some _ => State (Some mainC) [] init_procs
-    | None   => State None         [] init_procs
-    end.
-
-  Definition cur_comp (e: event) : Component.id :=
-    match e with
-    | ECall C _ _ _ => C
-    | ERet  C _ _   => C
+    | Some _ => State (Some (mainC, O)) []
+    | None   => State None              []
     end.
 
   (** Given the current event and the call stack, compute the next value of
       cur_proc. *)
-  Definition next_proc (e: event) (callers: list (option Procedure.id)) : option Procedure.id :=
+  Definition next_comp
+    (e: event)
+    (callers: list (Component.id * nat))
+    : option (Component.id * nat) :=
     match e with
     | ECall _ next_proc _ next_comp =>
       match PMap.find next_comp ictx with
-      | Some _ => Some next_proc
+      | Some _ => Some (next_comp, O)
       | None   => None
       end
     | ERet _ _ next_comp =>
-      match callers with
-      | [] => (* Should never happen *) None
-      | next_proc :: callers' =>
-        match PMap.find next_comp ictx with
-        | Some _ => next_proc
-        | None   => None
-        end
+      match PMap.find next_comp ictx, callers with
+      | Some _, (C, n) :: callers' => Some (C, S n)
+      | Some _, []                 => (* Should never happen *) None
+      | None  , _                  => None
       end
     end.
 
   (** Compute the next value of callers. *)
   Definition next_callers
     (e: event)
-    (cur_proc: option Procedure.id)
-    (callers: list (option Procedure.id)) : list (option Procedure.id) :=
+    (cur_proc: option (Component.id * nat))
+    (callers: list (Component.id * nat))
+    : list (Component.id * nat) :=
     match e with
-    | ECall _ _ _ _ => cur_proc :: callers
-    | ERet _ _ _ => tail callers
+    | ECall _ _ _ _ =>
+      match cur_proc with
+      | Some cur_proc => cur_proc :: callers
+      | None          => callers
+      end
+    | ERet _ _ next_comp =>
+      match PMap.find next_comp ictx with
+      | Some _ => tail callers
+      | None   => callers
+      end
     end.
 
-  (** Given an event e, compute the expression needed to produce that event.
-      That expression will be added to the code of the current procedure
-      below. *)
-  Definition next_instr (e: event) : expr :=
+  Definition correct_event (e: event) (ps: state) :=
     match e with
-    | ECall _ next_proc arg next_comp =>
-      E_call next_comp next_proc (E_val (Int arg))
-    | ERet  _ ret_val _ => E_val (Int ret_val)
+    | ECall _ _ _ _ => True
+    | ERet  _ _ next_comp =>
+      match PMap.find next_comp ictx, (callers ps) with
+      | Some _, (C, _) :: callers' => next_comp = C
+      | Some _, []                 => False
+      | None  , _                  => True
+      end
     end.
 
   (** Update the state of the context building procedure with an event. *)
   Definition update_state (ps: state) (e: event) : state :=
-    let 'State cur_proc callers procs := ps in
-    (* Test whether the call was performed from the context *)
-    match PMap.find (cur_comp e) procs, cur_proc with
-    | Some (n_events, cur_comp_procs), Some cur_proc =>
-      (* If so, add a corresponding instruction to the code of the calling
-         procedure *)
-      match PMap.find cur_proc cur_comp_procs with
-      | Some code =>
-        {| cur_proc := next_proc e callers;
-           callers  := next_callers e (Some cur_proc) callers;
-           procs    :=
-             PMap.add (cur_comp e)
-                      (Z.succ n_events,
-                       PMap.add cur_proc (code ++ [(n_events, next_instr e)]) cur_comp_procs)
-                      procs |}
-      | None =>
-        (* This branch should never be executed, as there should be code for
-           all procedures present here. *)
-        ps
-      end
-    | _, _ =>
-      (* If not, simply update cur_proc and callers. *)
-      {| cur_proc := next_proc e callers;
-         callers  := next_callers e cur_proc callers;
-         procs    := procs |}
+    {| cur_comp := next_comp e (callers ps);
+       callers  := next_callers e (cur_comp ps) (callers ps) |}.
+
+  (** Given an event e, compute the expression needed to produce that event.
+      Note that calls are compiled to two call expressions: one that produces
+      the call event proper, and another one that performs a recursive call to
+      continue executing the rest of the instructions in this procedure. *)
+  Definition expr_of_event (C: Component.id) (P: Procedure.id) (e: event) : expr :=
+    match e with
+    | ECall _ next_proc arg next_comp =>
+      E_seq (E_call next_comp next_proc (E_val (Int arg)))
+            (E_call C P (E_val (Int 0)))
+    | ERet  _ ret_val _ => E_val (Int ret_val)
     end.
+
+  Definition switch_clause n e_then e_else :=
+    let one := E_val (Int 1%Z) in
+    let count := E_binop Add E_local one in
+    E_if (E_binop Eq (E_deref count) (E_val (Int n)))
+         (E_seq (E_assign count (E_binop Add (E_deref count) one)) e_then)
+         e_else.
+
+  Ltac take_step :=
+    eapply (@star_step _ _ _ _ _ E0 _ E0 _ E0); trivial; [econstructor|].
+
+  Lemma switch_clause_spec p' C stk mem b n n' e_then e_else :
+    PMap.find C (genv_buffers (globalenv (CS.sem p'))) = Some b ->
+    Memory.load mem (C, b, 1) = Some (Int n) ->
+    if n =? n' then
+      exists mem',
+        Memory.store mem (C, b, 1) (Int (Z.succ n)) = Some mem' /\
+        Star (CS.sem p')
+             (C, stk, mem , Kstop, switch_clause n' e_then e_else) E0
+             (C, stk, mem', Kstop, e_then)
+    else
+      Star (CS.sem p')
+           (C, stk, mem, Kstop, switch_clause n' e_then e_else) E0
+           (C, stk, mem, Kstop, e_else).
+  Proof.
+    intros Eb Hload.
+    destruct (Z.eqb_spec n n') as [n_n'|n_n'].
+    - subst n'.
+      assert (Hload' := Hload).
+      unfold Memory.load in Hload'.
+      unfold Memory.store.
+      destruct (PMap.find C mem) as [memC|] eqn:EmemC; try discriminate.
+      destruct (ComponentMemory.store_after_load _ _ _ _ (Int (Z.succ n)) Hload')
+        as [memC' EmemC'].
+      rewrite EmemC'.
+      eexists; split; eauto.
+      repeat take_step; trivial; try eassumption.
+      repeat take_step; trivial; try eassumption.
+      { rewrite Z.eqb_refl. discriminate. }
+      { unfold Memory.store. rewrite EmemC. simpl. now rewrite Z.add_1_r, EmemC'. }
+      apply star_refl.
+    - unfold switch_clause.
+      repeat take_step; trivial; try eassumption.
+      eapply (@star_step _ _ _ _ _ E0 _ E0 _ E0); trivial; simpl.
+      { rewrite <- Z.eqb_neq in n_n'. rewrite n_n'. simpl.
+        eapply CS.KS_IfFalse. }
+      apply star_refl.
+  Qed.
+
+  Definition switch_add_expr e res :=
+    (pred (fst res), switch_clause (Z.of_nat (fst res)) e (snd res)).
+
+  Definition switch (es: list expr) (e_else: expr) : expr :=
+    snd (fold_right switch_add_expr (pred (length es), e_else) es).
+
+  Lemma switch_spec_else p' C stk mem b n es e_else :
+    PMap.find C (genv_buffers (globalenv (CS.sem p'))) = Some b ->
+    Memory.load mem (C, b, 1) = Some (Int (Z.of_nat n)) ->
+    (length es <= n)%nat ->
+    Star (CS.sem p')
+         (C, stk, mem, Kstop, switch es e_else) E0
+         (C, stk, mem, Kstop, e_else).
+  Proof. Admitted.
+
+  Lemma switch_spec p' C stk mem b es e es' e_else :
+    PMap.find C (genv_buffers (globalenv (CS.sem p'))) = Some b ->
+    Memory.load mem (C, b, 1) = Some (Int (Z.of_nat (length es))) ->
+    exists mem',
+      Memory.store mem (C, b, 1) (Int (Z.of_nat (S (length es)))) = Some mem' /\
+      Star (CS.sem p')
+           (C, stk, mem , Kstop, switch (es ++ e :: es') e_else) E0
+           (C, stk, mem', Kstop, e).
+  Proof.
+    intros Eb Hload.
+    assert (Eswitch :
+              exists e_else',
+                switch (es ++ e :: es') e_else =
+                switch es (switch_clause (Z.of_nat (length es)) e e_else')).
+    { unfold switch. rewrite fold_right_app, app_length. simpl.
+      assert (Efst : fst (fold_right switch_add_expr (pred (length es + S (length es'))%nat, e_else) es')
+                     = length es).
+      { rewrite Nat.add_comm.
+        generalize (length es). simpl.
+        induction es' as [|e' es' IH]; try easy. simpl.
+        intros n. now rewrite <- Nat.add_succ_r, IH. }
+      exists (snd (fold_right switch_add_expr (pred (length es + S (length es'))%nat, e_else) es')).
+      repeat f_equal. rewrite surjective_pairing at 1. simpl. rewrite Efst. f_equal. }
+    destruct Eswitch as [e_else' ->]. clear e_else. rename e_else' into e_else.
+    assert (Hcont := switch_clause_spec stk (Z.of_nat (length es)) e e_else Eb Hload).
+    rewrite Z.eqb_refl in Hcont.
+    destruct Hcont as (mem' & Hstore & Hstar2).
+    exists mem'. rewrite Nat2Z.inj_succ. split; trivial.
+    apply (fun H => @star_trans _ _ _ _ _ E0 _ H E0 _ _ Hstar2); trivial.
+    apply (switch_spec_else stk _ Eb Hload).
+    reflexivity.
+  Qed.
+
+  (*
 
   (** After we apply update_state to all the events in the trace,
       linearize_instructions converts the representation of each procedure into
@@ -196,15 +272,15 @@ Section Definability.
   Definition linearize_instructions
     (C: Component.id)
     (P: Procedure.id)
-    (instrs: list (Z * expr)) : expr :=
+    (instrs: list event) : expr :=
     let one := E_val (Int 1%Z) in
     let count := E_binop Add E_local one in
-    let add_instruction p e :=
-        let '(pos, instr) := p in
+    let add_instruction p exp :=
+        let '(pos, e) := p in
         E_if (E_binop Eq count (E_val (Int pos)))
              (E_seq (E_assign count (E_binop Add (E_deref count) one))
-                    (E_seq instr (E_call C P one)))
-             e in
+                    (expr_of_event C P e))
+             exp in
     fold_right add_instruction E_exit instrs.
 
   (** Combine all of the above steps to convert a trace into a context. *)
@@ -221,6 +297,71 @@ Section Definability.
        prog_buffers    := comp_mem;
        prog_main       := (mainC, mainP) |}.
 
+  Definition represent_cur_comp (g: global_env) (ps: state) (s: PS.state) : Prop :=
+    match cur_proc ps, s with
+    | Some (cur_comp, P), PS.PC (C, _, _, k, exp) =>
+      C = cur_comp /\
+      k = Kstop    /\
+      exists C_procs,
+        PMap.find C (genv_procedures g) = Some C_procs /\
+        PMap.find P C_procs             = Some exp
+    | None              , PS.CC _               => True
+    | _                 , _                     => False
+    end.
+
+  Definition represent_mem (g: global_env) (ps: state) (s: PS.state) : Prop :=
+    match s with
+    | PS.PC (_, _, mem, _, _)
+    | PS.CC (_, _, mem) =>
+      forall C : Component.id,
+        match PMap.find C (procs ps), PMap.find C (genv_buffers g), PMap.find C mem with
+        | Some (n_ps, _), Some b, Some C_mem =>
+          match ComponentMemory.load C_mem b 1 with
+          | Some n_s => n_s = Int n_ps
+          | None     => False
+          end
+        | None, _, None => True
+        | _, _, _ => False
+        end
+    end.
+
+  Definition represent_state (g: global_env) (prefix suffix: trace) (s: PS.state) : Prop :=
+    let ps := fold_left update_state prefix initial_state in
+    represent_cur_comp g ps s /\
+    represent_mem g ps s.
+
+  Lemma preservation g prefix e suffix s :
+    represent_state g prefix (e :: suffix) s ->
+    exists s',
+      step (PS.sem (build_context (prefix ++ e :: suffix)) (prog_interface p)) g s [e] s' /\
+      represent_state g (prefix ++ [e]) suffix s'.
+  Proof.
+    unfold represent_state.
+    intros [Hcur_comp Hmem].
+    destruct s as [[[[[C stack] mem] k] exp]|].
+    - (* s = PC (C, stack, mem, k, exp).  Note that, because of the switched
+         roles, this means that s is running the generated context program *)
+      unfold represent_cur_comp in Hcur_comp.
+      destruct (cur_proc (fold_left update_state prefix initial_state)) as [[C' P]|] eqn:Ecur_proc; try easy.
+      destruct Hcur_comp as (? & ? & C_procs & H1 & H2).
+      subst C' k.
+
+
+
+  Lemma context_definability_partial :
+    forall s t s',
+      Smallstep.initial_state (PS.sem p ictx) s ->
+      Star (PS.sem p ictx) s t s' ->
+      exists sctx sctx',
+      Star (PS.sem (build_context t) (prog_interface p)) sctx t sctx'.
+  Proof.
+    simpl.
+    intros s t s' Hinit.
+    destruct Hinit as [scs sps scs_sps init_scs].
+
+
+
+
   Theorem context_definability:
     forall t beh,
       program_behaves (PS.sem p ictx) (behavior_app t beh) ->
@@ -228,5 +369,11 @@ Section Definability.
       PMap.Equal (prog_interface ctx) ictx /\
       program_behaves (CS.sem (program_link p ctx mainC mainP)) (Terminates t).
   Proof.
-  Admitted.
+    intros t beh Hbeh.
+    remember (behavior_app t beh) as beh' eqn:E.
+    destruct Hbeh as [s beh' s_is_init s_beh|].
+    - (* Program has a valid initial state. *)
+      subst beh'.
+
+   *)
 End Definability.
